Refactor

src/localdrf/LocalDRF_Sim.v
@@ -89,8 +89,10 @@ Section SIM.
       (BOT: forall tid (NONE: IdentMap.find tid ths_src = None),
           (<<PROM: forall loc ts, ~ prom tid loc ts>>) /\
           (<<EXTRA: forall loc ts from, ~ extra tid loc ts from>>))
-      (MEMPF: sim_memory L times (all_promises (fun _ => True)prom) (all_extra (fun _ => True) extra) mem_mid mem_tgt)
+      (MEMPF: sim_memory L times (all_promises (fun _ => True) prom) (all_extra (fun _ => True) extra) mem_mid mem_tgt)
       (SCPF: TimeMap.le sc_src sc_tgt)
+
+      (JOINED: forall loc ts (NLOC: ~ L loc), List.Forall (fun vw => Memory.closed_view vw mem_src) (views loc ts))
       (MEMJOIN: SimMemory.sim_memory mem_mid mem_tgt)
       (MEMWF: memory_times_wf times mem_mid)
       (CONSISTENT: True)
@@ -103,15 +105,86 @@ Section SIM.
   .
   Hint Constructors sim_configuration.
 
+  Inductive sim_thread
+            (views: Loc.t -> Time.t -> list View.t)
+            (prom_self prom_others: Loc.t -> Time.t -> Prop)
+            (extra_self extra_others: Loc.t -> Time.t -> Time.t -> Prop):
+    forall lang (th_src th_mid th_tgt: Thread.t lang), Prop :=
+  | sim_thread_intro
+      lang st lc_src lc_mid lc_tgt
+      mem_src mem_mid mem_tgt sc_src sc_tgt
+      (LOCALPF: JSim.sim_local views lc_src lc_mid)
+      (LOCALJOIN: sim_local L times prom_self extra_self lc_mid lc_tgt)
+      (MEMPF: SimMemory.sim_memory mem_src mem_mid)
+      (MEMJOIN: sim_memory L times (prom_self \\2// prom_others) (extra_self \\3// extra_others) mem_mid mem_tgt)
+      (SC: TimeMap.le sc_src sc_tgt)
+    :
+      sim_thread
+        views prom_self prom_others extra_self extra_others
+        (Thread.mk lang st lc_src sc_src mem_src)
+        (Thread.mk lang st lc_mid sc_src mem_mid)
+        (Thread.mk lang st lc_tgt sc_tgt mem_tgt)
+  .
+  Hint Constructors sim_thread.
+
+  Lemma sim_thread_step
+        views0 prom_self0 prom_others extra_self0 extra_others
+        lang th_src0 th_mid0 th_tgt0 th_tgt1 pf_tgt e_tgt
+        (STEPTGT: Thread.step pf_tgt e_tgt th_tgt0 th_tgt1)
+        (NOREAD: no_read_msgs prom_others e_tgt)
+        (EVENT: ThreadEvent.get_machine_event e_tgt = MachineEvent.silent)
+
+        (THREAD: @sim_thread
+                   views0 prom_self0 prom_others extra_self0 extra_others
+                   lang th_src0 th_mid0 th_tgt0)
+
+        (SCSRC: Memory.closed_timemap th_src0.(Thread.sc) th_src0.(Thread.memory))
+        (SCMID: Memory.closed_timemap th_mid0.(Thread.sc) th_mid0.(Thread.memory))
+        (SCTGT: Memory.closed_timemap th_tgt0.(Thread.sc) th_tgt0.(Thread.memory))
+        (MEMSRC: Memory.closed th_src0.(Thread.memory))
+        (MEMMID: Memory.closed th_mid0.(Thread.memory))
+        (MEMTGT: Memory.closed th_tgt0.(Thread.memory))
+        (LOCALSRC: Local.wf th_src0.(Thread.local) th_src0.(Thread.memory))
+        (LOCALMID: Local.wf th_mid0.(Thread.local) th_mid0.(Thread.memory))
+        (LOCALTGT: Local.wf th_tgt0.(Thread.local) th_tgt0.(Thread.memory))
+
+        (MEMWF: memory_times_wf times th_mid0.(Thread.memory))
+        (CONSISTENT: Local.promise_consistent th_tgt0.(Thread.local))
+
+        (EXCLUSIVE: forall loc ts (OTHER: prom_others loc ts),
+            exists from msg, <<UNCH: unchangable th_src0.(Thread.memory) th_src0.(Thread.local).(Local.promises) loc ts from msg>>)
+        (EXCLUSIVEEXTRA: forall loc ts from (OTHER: extra_others loc ts from),
+            (<<UNCH: unchangable th_src0.(Thread.memory) th_src0.(Thread.local).(Local.promises) loc ts from Message.reserve>>))
+        (JOINED: forall loc ts (NLOC: ~ L loc), List.Forall (fun vw => Memory.closed_view vw th_src0.(Thread.memory)) (views0 loc ts))
+
+        (REL: joined_released
+                views0 th_mid0.(Thread.local).(Local.promises) th_mid0.(Thread.local).(Local.tview).(TView.rel))
+        (JOINEDMEM: joined_memory views0 th_mid0.(Thread.memory))
+        (VIEWS: wf_views views0)
+    :
+      exists th_mid1 th_src1 views1 prom_self1 extra_self1 pf_mid e_mid tr,
+        (<<STEPMID: JThread.step pf_mid e_mid th_mid0 th_mid1 views0 views1>>) /\
+        (<<STEPSRC: Trace.steps tr th_src0 th_src1>>) /\
+        (<<THREAD: sim_thread
+                     views1 prom_self1 prom_others extra_self1 extra_others
+                     th_src1 th_mid1 th_tgt1>>) /\
+        (<<EVENT: JSim.sim_event e_mid e_tgt>>) /\
+        (<<JOINED: forall loc ts (NLOC: ~ L loc), List.Forall (fun vw => Memory.closed_view vw th_src1.(Thread.memory)) (views1 loc ts)>>) /\
+        (<<TRACE: sim_silent_trace L tr (Some e_mid)>>).
+  Proof.
+  Admitted.
+
+
   Lemma step_sim_configuration views0 prom0 extra0
-        c_src0 c_mid0 c_tgt0 c_tgt1 e tid
-        (STEP: times_configuration_step times e tid c_tgt0 c_tgt1)
+        c_src0 c_mid0 c_tgt0 c_tgt1 e tid lang tr tr_cert
+        (STEP: @times_configuration_step times lang tr tr_cert e tid c_tgt0 c_tgt1)
+        (NOREAD: no_read_msgs
+
         (SIM: sim_configuration views0 prom0 extra0 c_src0 c_mid0 c_tgt0)
 
         (WF_SRC: Configuration.wf c_src0)
         (WF_MID: JConfiguration.wf views0 c_mid0)
         (WF_TGT: Configuration.wf c_tgt0)
-        (MEMWF: memory_times_wf times c_mid0.(Configuration.memory))
     :
       exists c_src1 c_mid1 views1 prom1 extra1,
         (<<STEP: JConfiguration.step e tid c_src0 c_src1 views0 views1>>) /\
