src/localdrf/TimeTraced.v
@@ -30,35 +30,42 @@ Set Implicit Arguments.
 
 
 Inductive times_configuration_step (times: Loc.t -> Time.t -> Prop)
-  : forall (e:MachineEvent.t) (tid:Ident.t) (c1 c2:Configuration.t), Prop :=
-| times_step_intro
-    lang tr e tr' pf tid c1 st1 lc1 e2 st3 lc3 sc3 memory3
+  : forall lang (tr tr_cert: Trace.t lang)
+           (e:MachineEvent.t) (tid:Ident.t) (c1 c2:Configuration.t), Prop :=
+| times_configuration_step_intro
+    lang tr e tr' pf tid c1 st1 lc1 e2 st3 lc3 sc3 memory3 tr_cert
     (TID: IdentMap.find tid c1.(Configuration.threads) = Some (existT _ lang st1, lc1))
     (STEPS: Trace.steps tr' (Thread.mk _ st1 lc1 c1.(Configuration.sc) c1.(Configuration.memory)) e2)
     (SILENT: List.Forall (fun the => ThreadEvent.get_machine_event (snd the) = MachineEvent.silent) tr')
     (STEP: Thread.step pf e e2 (Thread.mk _ st3 lc3 sc3 memory3))
     (TR: tr = tr'++[(e2, e)])
     (CONSISTENT: forall (EVENT: e <> ThreadEvent.failure),
-        exists times_cert tr_cert,
-          (<<CONSISTENT: pf_consistent_super_strong
-                           (Thread.mk _ st3 lc3 sc3 memory3)
-                           times_cert
-                           tr_cert times>>))
+        pf_consistent_super_strong (Thread.mk _ st3 lc3 sc3 memory3) tr_cert times)
+    (CERTNIL: e = ThreadEvent.failure -> tr_cert = [])
     (TIMES: List.Forall (fun thte => wf_time_evt times (snd thte)) tr)
   :
     times_configuration_step
-      times (ThreadEvent.get_machine_event e) tid c1 (Configuration.mk (IdentMap.add tid (existT _ _ st3, lc3) c1.(Configuration.threads)) sc3 memory3)
+      times tr tr_cert
+      (ThreadEvent.get_machine_event e) tid c1 (Configuration.mk (IdentMap.add tid (existT _ _ st3, lc3) c1.(Configuration.threads)) sc3 memory3)
 .
 
-Lemma times_configuration_step_traced_step times e tid c1 c2
-      (STEP: times_configuration_step times e tid c1 c2)
+Inductive times_configuration_step_all (times: Loc.t -> Time.t -> Prop)
+          (e:MachineEvent.t) (tid:Ident.t) (c1 c2:Configuration.t): Prop :=
+| times_configuration_step_all_intro
+    lang tr tr_cert
+    (STEP: @times_configuration_step times lang tr tr_cert e tid c1 c2)
+.
+
+Lemma times_configuration_step_traced_step times lang tr tr_cert e tid c1 c2
+      (STEP: @times_configuration_step times lang tr tr_cert e tid c1 c2)
       (WF: Configuration.wf c1)
   :
     exists lang (tr: Trace.t lang),
       (<<STEP: Trace.configuration_step tr e tid c1 c2>>).
 Proof.
-  inv STEP. esplits. econs; eauto.
-  i. exploit CONSISTENT; eauto. i. des.
+  inv STEP. apply inj_pair2 in H1. apply inj_pair2 in H2. subst.
+  esplits. econs; eauto.
+  i. hexploit CONSISTENT; eauto. i. des.
   dup WF. inv WF. exploit Trace.steps_future; eauto.
   { ss. eapply WF1; eauto. } i. des. ss.
   hexploit Trace.steps_future; eauto.
@@ -68,8 +75,8 @@ Proof.
 Qed.
 
 Lemma times_configuration_step_future
-      times e tid c1 c2
-      (STEP: times_configuration_step times e tid c1 c2)
+      times lang tr tr_cert e tid c1 c2
+      (STEP: @times_configuration_step times lang tr tr_cert e tid c1 c2)
       (WF1: Configuration.wf c1):
   (<<WF2: Configuration.wf c2>>) /\
   (<<SC_FUTURE: TimeMap.le c1.(Configuration.sc) c2.(Configuration.sc)>>) /\
@@ -82,58 +89,34 @@ Qed.
 Lemma times_configuration_step_mon times0 times1
       (LE: times0 <2= times1)
   :
-    times_configuration_step times0 <4= times_configuration_step times1.
+    times_configuration_step times0 <7= times_configuration_step times1.
 Proof.
-  i. inv PR. econs; eauto.
-  { i. exploit CONSISTENT; eauto. i. des. esplits; eauto.
+  i. inv PR. eapply inj_pair2 in H1. eapply inj_pair2 in H2. subst. econs; eauto.
+  { i. hexploit CONSISTENT; eauto. i. des. esplits; eauto.
     eapply pf_consistent_super_strong_mon; eauto. }
   { eapply List.Forall_impl; eauto. i. eapply wf_time_evt_mon; eauto. }
 Qed.
 
-Lemma event_times_list_exists
-      e
+Lemma times_configuration_step_all_mon times0 times1
+      (LE: times0 <2= times1)
   :
-    exists (times: Loc.t -> list Time.t),
-      (<<EVT: wf_time_evt (fun loc ts => List.In ts (times loc)) e >>).
+    times_configuration_step_all times0 <4= times_configuration_step_all times1.
 Proof.
-  destruct e; ss; try by (exists (fun _ => []); splits; auto).
-  { exists (fun loc' => if Loc.eq_dec loc' loc then [from; to] else []).
-    des_ifs; ss; auto. }
-  { exists (fun loc' => if Loc.eq_dec loc' loc then [from; to] else []).
-    des_ifs; ss; auto. }
-  { exists (fun loc' => if Loc.eq_dec loc' loc then [tsr; tsw] else []).
-    des_ifs; ss; auto. }
-Qed.
-
-Lemma trace_fin_events lang (tr: Trace.t lang)
-  :
-    exists (times: Loc.t -> list Time.t),
-      (<<TIMES: List.Forall (fun thte => wf_time_evt (fun loc ts => List.In ts (times loc)) (snd thte)) tr>>).
-Proof.
-  induction tr.
-  { exists (fun _ => []). ss. }
-  { des. hexploit (event_times_list_exists (snd a)). i. des.
-    exists (fun loc => times loc ++ times0 loc). econs.
-    { eapply wf_time_evt_mon; eauto. i. ss.
-      eapply List.in_or_app; auto. }
-    { eapply List.Forall_impl; eauto. i. ss.
-      eapply wf_time_evt_mon; eauto. i. ss.
-      eapply List.in_or_app; auto. }
-  }
+  i. inv PR. econs. eapply times_configuration_step_mon; eauto.
 Qed.
 
 Lemma times_configuration_step_exists c0 c1 tid e
       (STEP: Configuration.step e tid c0 c1)
       (WF: Configuration.wf c0)
   :
-    exists times,
-      (<<STEP: times_configuration_step times e tid c0 c1>>) /\
+    exists lang times tr tr_cert,
+      (<<STEP: @times_configuration_step times lang tr tr_cert e tid c0 c1>>) /\
       (<<WO: forall loc, well_ordered (times loc)>>).
 Proof.
   eapply Trace.step_configuration_step in STEP. des.
-  hexploit (trace_fin_events tr). i. des. inv STEP0.
+  hexploit (trace_times_list_exists tr). i. des. inv STEP0.
   eapply inj_pair2 in H1. subst. destruct (classic (e0 = ThreadEvent.failure)).
-  { subst. exists (fun loc ts => List.In ts (times loc)). splits.
+  { subst. eexists lang, (fun loc ts => List.In ts (times loc)), (tr'++_), []. splits.
     { econs; eauto. ss. }
     { i. eapply finite_well_ordered. }
   }
@@ -142,10 +125,11 @@ Proof.
     { ss. eapply WF1; eauto. } i. des. ss.
     hexploit Thread.step_future; eauto. i. des. ss.
     eapply consistent_pf_consistent_super_strong in H0; eauto.
-    des. exists (certimes \2/ (fun loc ts => List.In ts (times loc))). splits.
+    des. eexists lang, (certimes \2/ (fun loc ts => List.In ts (times loc))), (tr'++_), tr. splits.
     { econs; eauto.
       { i. esplits. eapply pf_consistent_super_strong_mon; eauto. }
-      { eapply List.Forall_impl; try apply TIMES.
+      { i. ss. }
+      { eapply List.Forall_impl; try apply WFTIME.
         i. ss. eapply wf_time_evt_mon; try apply H0. i. ss. auto. }
     }
     { i. eapply join_well_ordered; eauto. eapply finite_well_ordered. }
@@ -157,7 +141,7 @@ Lemma times_configuration_step_same_behaviors c beh
       (BEH: behaviors Configuration.step c beh)
   :
     exists times,
-      (<<BEH: behaviors (times_configuration_step times) c beh>>) /\
+      (<<BEH: behaviors (times_configuration_step_all times) c beh>>) /\
       (<<WO: forall loc, well_ordered (times loc)>>).
 Proof.
   ginduction BEH.
@@ -170,22 +154,22 @@ Proof.
     exploit times_configuration_step_exists; eauto. i. des.
     exists (times \2/ times0). splits.
     { econs 2; eauto.
-      { eapply times_configuration_step_mon; eauto. }
+      { econs. eapply times_configuration_step_mon; eauto. }
       { eapply le_step_behavior_improve; try apply BEH0.
-        eapply times_configuration_step_mon. i. auto. }
+        eapply times_configuration_step_all_mon; auto. }
     }
     { i. eapply join_well_ordered; eauto. }
   }
   { i. exploit times_configuration_step_exists; eauto. i. des.
-    exists times. splits; eauto. econs 3; eauto. }
+    exists times. splits; eauto. econs 3; eauto. econs; eauto. }
   { i. exploit IHBEH.
     { eapply Configuration.step_future; eauto. } i. des.
     exploit times_configuration_step_exists; eauto. i. des.
     exists (times \2/ times0). splits.
     { econs 4; eauto.
-      { eapply times_configuration_step_mon; eauto. }
+      { econs. eapply times_configuration_step_mon; eauto. }
       { eapply le_step_behavior_improve; try apply BEH0.
-        eapply times_configuration_step_mon. i. auto. }
+        eapply times_configuration_step_all_mon; auto. }
     }
     { i. eapply join_well_ordered; eauto. }
   }
